feat: Encryption Context and Encrypted Data Keys
Update the way Encryption Context
and Encrypted Data Keys are read and written.

src/SDK/Serialize/SerializeFunctions.dfy
@@ -5,104 +5,101 @@ include "../../../libraries/src/Collections/Sequences/Seq.dfy"
 include "../../Generated/AwsCryptographicMaterialProviders.dfy"
 include "../../StandardLibrary/StandardLibrary.dfy"
 include "../../Util/UTF8.dfy"
-include "./SerializableTypes.dfy"
 
 module SerializeFunctions {
   import opened Aws.Crypto
   import opened Seq
-  import opened SerializableTypes
   import opened StandardLibrary.UInt
   import opened Wrappers
   import opened UTF8
 
-  function method EncryptedDataKeysToSeq(edks: ESDKEncryptedDataKeys):  (ret: seq<uint8>)
+  datatype ReadProblems =
+    | MoreNeeded(pos: nat)
+    | Error(message: string)
+  type MoreNeeded = p: ReadProblems | p.MoreNeeded? witness *
+
+  // Think about a type
+  // datatype Thing = Thing(data: s:seq<uint8>, pos: nat)
+  // Then we take and return this thing,
+  // not just `pos`.
+  type ReadResult<T, E> = Result<(T, nat), E>
+  type ReadCorrect<T> = ReadResult<T, ReadProblems>
+  type ReadBinary<T> = ReadResult<T, MoreNeeded>
+
+  predicate CorrectlyRead<T> (
+    s: seq<uint8>,
+    pos: nat,
+    res: ReadCorrect<T>,
+    invertT: T -> seq<uint8>
+  )
   {
-    UInt16ToSeq(|edks| as uint16) + FoldLeft(FoldEncryptedDataKey, [], edks)
+    res.Success?
+    ==>
+      && |s| >= res.value.1 >= pos
+      && invertT(res.value.0) == s[pos..res.value.1]
   }
 
-  function method FoldEncryptedDataKey(acc: seq<uint8>, edk: ESDKEncryptedDataKey): (ret: seq<uint8>)
+  function method Read(
+    s: seq<uint8>,
+    pos: nat,
+    l: nat
+  ):
+    (res: ReadBinary<seq<uint8>>)
+    decreases if pos > 0 then true else false
+    requires l > 0
+    ensures
+      && |s| >= pos + l
+    ==>
+      && res.Success?
+      && |res.value.0| == l
+      && res.value.1 == pos + l >= 0
+      && |s| >= res.value.1 > pos
+      && s[pos..res.value.1] == res.value.0
+    ensures
+      && pos + l > |s|
+    ==>
+      && res.Failure?
+      && res.error.MoreNeeded?
+      && res.error.pos == pos + l
+    ensures CorrectlyRead(s, pos, res, d => d)
   {
-      acc
-        + UInt16ToSeq(|edk.keyProviderId| as uint16) + edk.keyProviderId
-        + UInt16ToSeq(|edk.keyProviderInfo| as uint16) + edk.keyProviderInfo
-        + UInt16ToSeq(|edk.ciphertext| as uint16) + edk.ciphertext
+    var end := pos + l;
+    if |s| >= end then
+      Success((s[pos..end], end))
+    else
+      Failure(MoreNeeded(end))
+  }
+
+  // Opaque? Because the body is not interesting...
+  function method ReadUInt16(
+    s: seq<uint8>,
+    pos: nat
+  ):
+    (res: ReadBinary<uint16>)
+    // decreases if pos > 0 then true else false
+    ensures CorrectlyRead(s, pos, res, UInt16ToSeq)
+  {
+    var (data, end) :- Read(s, pos, 2);
+    Success((SeqToUInt16(data), end))
+  }
+
+  function method WriteShortLengthSeq(
+    d: Uint8Seq16
+  ):
+    (res: seq<uint8>)
+  {
+    UInt16ToSeq(|d| as uint16) + d
   }
 
   function method ReadShortLengthSeq(
     s: seq<uint8>,
     pos: nat
-  ): (
-    Result<Option<(Uint8Seq16, nat)>, string>
-  ) {
-    if |s| >= pos+2 then
-      var length := SeqToUInt16(s[pos..2+pos]) as nat;
-      if |s| >= pos+2+length then
-        Success(Some((s[2+pos..2+pos+length], 2+pos+length)))
-      else
-        Success(None)
-    else
-      Success(None)
-  }
-
-  function method ReadEncryptedDataKey(s: seq<uint8>, pos: nat): Result<Option<(ESDKEncryptedDataKey, nat)>, string> {
-    var providerIDM :- ReadShortLengthSeq(s, pos);
-    match providerIDM {
-      case None => Success(None)
-      case Some((providerID, readProviderID)) =>
-        :- Need(ValidUTF8Seq(providerID), "Invalid providerID");
-        var providerInfoM :- ReadShortLengthSeq(s, readProviderID);
-        match providerIDM {
-          case None => Success(None)
-          case Some((providerInfo, readProviderInfo)) =>
-            var cipherTextM :- ReadShortLengthSeq(s, readProviderInfo);
-            match cipherTextM {
-              case None => Success(None)
-              case Some((cipherText, readCipherText)) =>
-                Success(Some((EncryptedDataKey(
-                  keyProviderId := providerID,
-                  keyProviderInfo := providerInfo,
-                  ciphertext := cipherText
-                ), readCipherText)))
-            }
-        }
-    }
-  }
-
-  function method ReadEncryptedDataKeyRecursive(s: seq<uint8>, pos: nat, remaining: uint16): (ret: Result<Option<(ESDKEncryptedDataKeys, nat)>, string>)
-    decreases remaining
-    ensures match ret
-      case Success(Some((edks, _))) => |edks| == remaining as int
-      case _ => true
+  ):
+    (res: ReadCorrect<Uint8Seq16>)
+    ensures CorrectlyRead(s, pos, res, WriteShortLengthSeq)
   {
-    match remaining {
-      case 0 =>
-        var r : ESDKEncryptedDataKeys := [];
-        Success(Some((r, pos)))
-      case _ =>
-        var edkM :- ReadEncryptedDataKey(s, pos);
-        match edkM {
-          case None => Success(None)
-          case Some((edk, newPos)) =>
-            var restM :- ReadEncryptedDataKeyRecursive(s, newPos, remaining - 1);
-            match restM {
-              case None =>
-                Success(None)
-              case Some((restEDKs, restPos)) =>
-                var edks : ESDKEncryptedDataKeys := [edk] + restEDKs;
-                Success(Some((edks, restPos)))
-            }
-        }
-    }
-  }
-
-  function method EncryptedDataKeysFromSeq(s: seq<uint8>, pos: nat): Result<Option<(ESDKEncryptedDataKeys, nat)>, string> {
-    if |s| >= pos+2 then
-      var count := SeqToUInt16(s[pos..2+pos]);
-      if count == 0 then
-        Failure("Invalid EDKs seq")
-      else
-        ReadEncryptedDataKeyRecursive(s, pos+2, count)
-    else
-      Success(None)
+    var (length, dataPos) :- ReadUInt16(s, pos);
+    :- Need(length > 0, Error("Length cannot be 0."));
+    Read(s, dataPos, length as nat)
   }
 }
