src/SDK/Serialize/EncryptedDataKeys.dfy
@@ -1,0 +1,105 @@
+// Copyright Amazon.com Inc. or its affiliates. All Rights Reserved.
+// SPDX-License-Identifier: Apache-2.0
+
+include "../../../libraries/src/Collections/Sequences/Seq.dfy"
+include "../../Generated/AwsCryptographicMaterialProviders.dfy"
+include "../../StandardLibrary/StandardLibrary.dfy"
+include "../../Util/UTF8.dfy"
+include "./SerializableTypes.dfy"
+include "SerializeFunctions.dfy"
+
+module EncryptedDataKeys {
+  import Aws.Crypto
+  import Seq
+  import opened SerializableTypes
+  import opened StandardLibrary.UInt
+  import opened Wrappers
+  import opened UTF8
+  import opened SerializeFunctions
+
+  function method WriteEncryptedDataKey(edk: ESDKEncryptedDataKey): (ret: seq<uint8>)
+  {
+    WriteShortLengthSeq(edk.keyProviderId)
+    + WriteShortLengthSeq(edk.keyProviderInfo)
+    + WriteShortLengthSeq(edk.ciphertext)
+  }
+
+  function method {:tailrecursion} WriteEncryptedDataKeys(
+    edks: ESDKEncryptedDataKeys
+  ):
+    (ret: seq<uint8>)
+    ensures |edks| == 0 ==> ret == []
+    ensures |edks| != 0
+    ==>
+      WriteEncryptedDataKeys(Seq.DropLast(edks))
+        + WriteEncryptedDataKey(Seq.Last(edks))
+      == ret
+  {
+    if |edks| == 0 then []
+    else
+      WriteEncryptedDataKeys(Seq.DropLast(edks)) + WriteEncryptedDataKey(Seq.Last(edks))
+  }
+
+  function method WriteEncryptedDataKeysSection(
+    edks: ESDKEncryptedDataKeys
+  ):
+    (ret: seq<uint8>)
+  {
+    UInt16ToSeq(|edks| as uint16) + WriteEncryptedDataKeys(edks)
+  }
+
+  function method ReadEncryptedDataKey(
+    s: seq<uint8>,
+    pos: nat
+  ):
+    (res: ReadCorrect<ESDKEncryptedDataKey>)
+    ensures CorrectlyRead(s, pos, res, WriteEncryptedDataKey)
+  {
+    var (providerId, providerIdPos) :- ReadShortLengthSeq(s, pos);
+    :- Need(ValidUTF8Seq(providerId), Error("Invalid providerID"));
+    var (providerInfo, providerInfoPos) :- ReadShortLengthSeq(s, providerIdPos);
+    var (cipherText, cipherTextPos) :- ReadShortLengthSeq(s, providerInfoPos);
+    var edk: ESDKEncryptedDataKey := Crypto.EncryptedDataKey(
+        keyProviderId := providerId,
+        keyProviderInfo := providerInfo,
+        ciphertext := cipherText);
+
+    Success((edk, cipherTextPos))
+  }
+
+  function method {:tailrecursion true} ReadEncryptedDataKeys(
+    s: seq<uint8>,
+    pos: nat,
+    acc: ESDKEncryptedDataKeys,
+    count: uint16,
+    nextEdk: nat
+  ):
+    (res: ReadCorrect<ESDKEncryptedDataKeys>)
+    requires 0 <= |acc| <= count as nat < UINT16_LIMIT
+    requires |s| >= nextEdk >= pos
+    requires WriteEncryptedDataKeys(acc) == s[pos..nextEdk]
+    decreases count as int - |acc|
+    ensures CorrectlyRead(s, pos, res, WriteEncryptedDataKeys)
+    ensures res.Success? ==> count as nat == |res.value.0|
+  {
+    if count as int > |acc| then
+      var (edk, newPos) :- ReadEncryptedDataKey(s, nextEdk);
+      var nextAcc := acc + [edk];
+      ReadEncryptedDataKeys(s, pos, nextAcc, count, newPos)
+    else
+      Success((acc, nextEdk))
+  }
+
+  function method ReadEncryptedDataKeysSection(
+    s: seq<uint8>,
+    pos: nat
+  ):
+    (res: ReadCorrect<ESDKEncryptedDataKeys>)
+    ensures CorrectlyRead(s, pos, res, WriteEncryptedDataKeysSection)
+  {
+    var (count, edkStart) :- ReadUInt16(s, pos);
+    :- Need(count > 0, Error("Invalid EDKs seq"));
+    var (edks, end) :- ReadEncryptedDataKeys(s, edkStart, [], count, edkStart);
+    Success((edks, end))
+  }
+}
