src/SDK/Serialize/EncryptionContext.dfy
@@ -1,0 +1,379 @@
+// Copyright Amazon.com Inc. or its affiliates. All Rights Reserved.
+// SPDX-License-Identifier: Apache-2.0
+
+include "../../../libraries/src/Collections/Sequences/Seq.dfy"
+include "../../Generated/AwsCryptographicMaterialProviders.dfy"
+include "../../StandardLibrary/StandardLibrary.dfy"
+include "../../Util/UTF8.dfy"
+include "./SerializableTypes.dfy"
+include "SerializeFunctions.dfy"
+include "../../Util/Sets.dfy"
+
+module EncryptionContext2 {
+  import Aws.Crypto
+  import Seq
+  import StandardLibrary
+  import Sets
+  // import opened SerializableTypes
+  import opened StandardLibrary.UInt
+  import opened Wrappers
+  import opened UTF8
+  import opened SerializeFunctions
+
+  // There needs to be a canonical representation of the encryption context.
+  // Once the encryption context has been serialized,
+  // then the bytes in the message can provide this canonical representation.
+  // However, it is best if a canonical representation exists.
+  // For reading and writing, we use the arbitrary given order,
+  // and separate the ordering problem from serialization.
+
+  datatype Pair<K, V> = Pair(key: K, value: V)
+  type Linear<K, V> = seq<Pair<K,V>>
+
+  type ESDKEncryptionContextPair = p: Pair<UTF8.ValidUTF8Bytes, UTF8.ValidUTF8Bytes>
+  |
+    && HasUint16Len(p.key) && ValidUTF8Seq(p.key)
+    && HasUint16Len(p.value) && ValidUTF8Seq(p.value)
+  witness *
+
+  const ESDK_CANONICAL_ENCRYPTION_CONTEXT_MAX_LENGTH := UINT16_LIMIT - 2;
+  type SeqEcMaxBytes = s: seq<uint8>
+  | |s| < ESDK_CANONICAL_ENCRYPTION_CONTEXT_MAX_LENGTH
+  witness *
+
+  type ESDKCanonicalEncryptionContext = pairs: seq<ESDKEncryptionContextPair>
+  |
+    && HasUint16Len(pairs)
+    && LinearLength2(pairs) < ESDK_CANONICAL_ENCRYPTION_CONTEXT_MAX_LENGTH
+    //= compliance/data-format/message-header.txt#2.5.1.7.2.2
+    //= type=implication
+    //# This sequence MUST NOT contain duplicate entries.
+    && KeysAreUnique(pairs)
+  witness *
+
+  predicate KeysAreUnique<K, V>(pairs: Linear<K, V>)
+  {
+    (forall i, j
+    ::
+      && 0 <= i < |pairs|
+      && 0 <= j < |pairs|
+      && i != j
+    ==> pairs[i].key != pairs[j].key)
+  }
+
+  function method {:vcs_split_on_every_assert} CanonicalEncryptionContext(
+    encryptionContext: ESDKEncryptionContext
+  )
+    :(ret: ESDKCanonicalEncryptionContext)
+  {
+    //= compliance/data-format/message-header.txt#2.5.1.7.2.2
+    //# These entries MUST have entries sorted, by key, in ascending order
+    //# according to the UTF-8 encoded binary value.
+    var keys: seq<UTF8.ValidUTF8Bytes> := Sets.ComputeSetToOrderedSequence<uint8>(
+      encryptionContext.Keys,
+      UInt.UInt8Less
+    );
+    seq(
+      |keys|,
+      i
+        requires 0 <= i < |keys|
+      => Pair(
+        keys[i],
+        encryptionContext[keys[i]]))
+  }
+
+  function method EncryptionContext(
+    canonicalEncryptionContext: ESDKCanonicalEncryptionContext
+  )
+    :(ret: Crypto.EncryptionContext)
+  {
+    // This is needed because Dafny can not reveal the subset type by default?
+    assert KeysAreUnique(canonicalEncryptionContext);
+    map p: ESDKEncryptionContextPair
+    | p in canonicalEncryptionContext
+    :: p.key := p.value
+  }
+
+  //= compliance/data-format/message-header.txt#2.5.1.7
+  //# The following table describes the fields that form the AAD.  The
+  //# bytes are appended in the order shown.
+  //# 
+  //#  +=================+==============================+================+
+  //#  | Field           | Length (bytes)               | Interpreted as |
+  //#  +=================+==============================+================+
+  //#  | Key Value Pairs | 2                            | UInt16         |
+  //#  | Length (Section |                              |                |
+  //#  | 2.5.1.7.1)      |                              |                |
+  //#  +-----------------+------------------------------+----------------+
+  //#  | Key Value Pairs | Variable.  Determined by the | Key Value      |
+  //#  | (Section        | value of Key Value Pairs     | Pairs (Section |
+  //#  | 2.5.1.7.2)      | Length (Section 2.5.1.7.1).  | 2.5.1.7.2)     |
+  //#  +-----------------+------------------------------+----------------+
+  function method WriteAADSection(
+    ec: ESDKCanonicalEncryptionContext
+  ):
+    (ret: seq<uint8>)
+    ensures |ec| == 0
+    ==>
+      // These all deal with |ec| == 0
+
+      //= compliance/data-format/message-header.txt#2.5.1.7.1
+      //= type=implication
+      //# When the encryption context (../framework/structures.md#encryption-
+      //# context) is empty, the value of this field MUST be 0.
+
+      //= compliance/data-format/message-header.txt#2.5.1.7.2
+      //= type=implication
+      //# When the encryption
+      //# context (../framework/structures.md#encryption-context) is empty,
+      //# this field MUST NOT be included in the Section 2.5.1.7.
+
+      //= compliance/data-format/message-header.txt#2.5.1.7.2.1
+      //= type=implication
+      //# The value of this field MUST be greater
+      //# than 0.
+      ret == UInt16ToSeq(0)
+    ensures |ec| != 0
+    ==>
+      && ret == UInt16ToSeq(|WriteAAD(ec)| as uint16)
+        + WriteAAD(ec)
+    {
+    if |ec| == 0 then UInt16ToSeq(0)
+    else
+      var aad := WriteAAD(ec);
+      UInt16ToSeq(|aad| as uint16) + aad
+  }
+
+  //= compliance/data-format/message-header.txt#2.5.1.7.2
+  //#The following table describes the fields that form the Key Value
+  //#Pairs.  The bytes are appended in the order shown.
+  //#
+  //#  +==================+=========================+==================+
+  //#  | Field            | Length (bytes)          | Interpreted as   |
+  //#  +==================+=========================+==================+
+  //#  | Key Value Pair   | 2                       | UInt16           |
+  //#  | Count (Section   |                         |                  |
+  //#  | 2.5.1.7.2.1)     |                         |                  |
+  //#  +------------------+-------------------------+------------------+
+  //#  | Key Value Pair   | Variable.  Determined   | Key Value Pair   |
+  //#  | Entries (Section | by the count and length | Entries (Section |
+  //#  | 2.5.1.7.2.2)     | of each key-value pair. | 2.5.1.7.2.2)     |
+  //#  +------------------+-------------------------+------------------+
+  function method WriteAAD(
+    ec: ESDKCanonicalEncryptionContext
+  ):
+    (ret: seq<uint8>)
+    ensures HasUint16Len(ret)
+    // To support older versions of the ESDK
+    // |ec| == 0 is encoded as 0 count.
+    // However, this is never called on write path.
+    // See WriteAADSection
+    ensures |ec| == 0 ==> ret == UInt16ToSeq(0)
+  {
+    if |ec| == 0 then UInt16ToSeq(0)
+    else 
+      UInt16ToSeq(|ec| as uint16) + WriteAADPairs(ec)
+  }
+
+  function method {:tailrecursion} WriteAADPairs(
+    ec: ESDKCanonicalEncryptionContext
+  ):
+    (ret: seq<uint8>)
+    ensures |ec| == 0
+    ==>
+      && LinearLength2(ec) == |ret|
+      && ret == []
+    ensures |ec| != 0
+    ==>
+      && LinearLength2(Seq.DropLast(ec)) + PairLength(Seq.Last(ec)) == |ret|
+      && WriteAADPairs(Seq.DropLast(ec)) + WriteAADPair(Seq.Last(ec)) == ret
+    ensures |ret| < ESDK_CANONICAL_ENCRYPTION_CONTEXT_MAX_LENGTH
+  {
+    if |ec| == 0 then []
+    else
+      assert LinearLength2(Seq.DropLast(ec)) < LinearLength2(ec);
+      WriteAADPairs(Seq.DropLast(ec)) + WriteAADPair(Seq.Last(ec))
+  }
+
+  //= compliance/data-format/message-header.txt#2.5.1.7.2.2
+  //# The following table describes the fields that form each key value
+  //# pair entry.  The bytes are appended in the order shown.
+  //# 
+  //# +========+=========================================+================+
+  //# | Field  | Length (bytes)                          | Interpreted    |
+  //# |        |                                         | as             |
+  //# +========+=========================================+================+
+  //# | Key    | 2                                       | UInt16         |
+  //# | Length |                                         |                |
+  //# +--------+-----------------------------------------+----------------+
+  //# | Key    | Variable.  Equal to the value specified | UTF-8 encoded  |
+  //# |        | in the previous 2 bytes (Key Length).   | bytes          |
+  //# +--------+-----------------------------------------+----------------+
+  //# | Value  | 2                                       | UInt16         |
+  //# | Length |                                         |                |
+  //# +--------+-----------------------------------------+----------------+
+  //# | Value  | Variable.  Equal to the value specified | UTF-8 encoded  |
+  //# |        | in the previous 2 bytes (Value Length). | bytes          |
+  //# +--------+-----------------------------------------+----------------+
+  function method WriteAADPair(
+    pair: ESDKEncryptionContextPair
+  ):
+    (ret: seq<uint8>)
+    ensures PairLength(pair) == |ret|
+  {
+    WriteShortLengthSeq(pair.key) + WriteShortLengthSeq(pair.value)
+  }
+
+  function method ReadAADPair(
+    s: seq<uint8>,
+    pos: nat
+  ):
+    (res: ReadCorrect<ESDKEncryptionContextPair>)
+    ensures CorrectlyRead(s, pos, res, WriteAADPair)
+  {
+    var (key, keyEnd) :- ReadShortLengthSeq(s, pos);
+    :- Need(ValidUTF8Seq(key), Error("Invalid Encryption Context key"));
+    var (value, end) :- ReadShortLengthSeq(s, keyEnd);
+    :- Need(ValidUTF8Seq(value), Error("Invalid Encryption Context value"));
+    Success((Pair(key, value), end))
+  }
+
+  function method {:tailrecursion} ReadAADPairs(
+    s: seq<uint8>,
+    pos: nat,
+    acc: ESDKCanonicalEncryptionContext,
+    keys: set<UTF8.ValidUTF8Bytes>,
+    count: uint16,
+    nextPair: nat
+  ):
+    (res: ReadCorrect<ESDKCanonicalEncryptionContext>)
+    requires 0 <= |acc| <= count as nat < UINT16_LIMIT
+    requires |s| >= nextPair >= pos
+    requires WriteAADPairs(acc) == s[pos..nextPair]
+    requires KeysToSet(acc) == keys
+    decreases count as int - |acc|
+    ensures res.Success?
+    ==>
+       && count as nat == |res.value.0|
+    ensures CorrectlyRead(s, pos, res, WriteAADPairs)
+  {
+    if count as int > |acc| then
+      var (pair, newPos) :- ReadAADPair(s, nextPair);
+      :- Need(pair.key !in keys, Error("Duplicate Encryption Context key value."));
+      :- Need(|s[pos..newPos]| < ESDK_CANONICAL_ENCRYPTION_CONTEXT_MAX_LENGTH, Error("Encryption Context exceeds maximum length."));
+
+      var nextAcc := acc + [pair];
+      var nextKeys := KeysToSet(nextAcc);
+      reveal KeysToSet();
+      assert KeysToSet(nextAcc) == KeysToSet(acc) + KeysToSet([pair]);
+      ReadAADPairs(s, pos, nextAcc, nextKeys, count, newPos)
+    else
+      assert WriteAADPairs(acc) == s[pos..nextPair];
+      Success((acc, nextPair))
+  }
+
+  function method ReadAAD(
+    s: seq<uint8>,
+    pos: nat
+  ):
+    (res: ReadCorrect<ESDKCanonicalEncryptionContext>)
+    ensures CorrectlyRead(s, pos, res, WriteAAD)
+  {
+    var (count, ecPos) :- ReadUInt16(s, pos);
+    if count == 0 then
+      var edks: ESDKCanonicalEncryptionContext := [];
+      Success((edks, ecPos))
+    else
+      var acc := [];
+      var keys := KeysToSet(acc);
+      ReadAADPairs(s, ecPos, acc, keys, count, ecPos)
+  }
+
+  function method ReadAADSection(
+    s: seq<uint8>,
+    pos: nat
+  ):
+    (res: ReadCorrect<ESDKCanonicalEncryptionContext>)
+    ensures
+      || CorrectlyRead(s, pos, res, WriteAADSection)
+      // This is an exceedingly rare case.
+      // The AAD section is supposed to encode
+      // an empty encryption context as a length of 0
+      // because the additional 2 bytes to encode 0 is redundant.
+      // However, since there did once exists ESDKs
+      // that incorrectly wrote empty encryption contexts as
+      // `[0,2,0,0]` this read path MUST be supported.
+      || (
+        && res.Success?
+        && pos+4 < |s|
+        && s[pos..pos+4] == [0,2,0,0]
+        ==>
+          && |res.value.0| == 0
+          && res.value.1 == pos + 4)
+  {
+    var (length: uint16, countPos: nat) :- ReadUInt16(s, pos);
+    if length == 0 then
+      Success(([], countPos))
+    else if countPos + length as nat < |s| then
+      Failure(MoreNeeded(countPos + length as nat))
+    else if length == 2 then
+      var (count, end) :- ReadUInt16(s, countPos);
+      :- Need(count == 0, Error("Encryption Context pairs count can not exceed byte length"));
+      Success(([], end))
+    else
+      var (count, _) :- ReadUInt16(s, countPos);
+      :- Need(count > 0, Error("Encryption Context byte length exceeds pairs count."));
+      ReadAAD(s, countPos)
+  }
+
+  function method {:opaque} KeysToSet<K(==), V(==)>(pairs: Linear<K, V>): set<K>
+  {
+    set p: Pair<K,V> | p in pairs :: p.key
+  }
+
+
+
+  // Copied from Serialized Types...
+
+  predicate method IsESDKEncryptionContext(ec: Crypto.EncryptionContext) {
+    && |ec| < UINT16_LIMIT
+    && Length2(ec) < UINT16_LIMIT
+    && forall element
+    | element in (multiset(ec.Keys) + multiset(ec.Values))
+    ::
+      && HasUint16Len(element)
+      && ValidUTF8Seq(element)
+  }
+
+  type ESDKEncryptionContext = ec: Crypto.EncryptionContext | IsESDKEncryptionContext(ec) witness *
+
+  function method Length2(encryptionContext: Crypto.EncryptionContext): nat
+  {
+    if |encryptionContext| == 0 then 0 else
+      // Defining and reasoning about order at this level is simplified by using a sequence of
+      // key value pairs instead of a map.
+      var keys: seq<UTF8.ValidUTF8Bytes> := Sets.ComputeSetToOrderedSequence<uint8>(encryptionContext.Keys, UInt.UInt8Less);
+      var pairs := seq(|keys|, i requires 0 <= i < |keys| => Pair(keys[i], encryptionContext[keys[i]]));
+      2 + LinearLength2(pairs)
+  }
+
+  function method LinearLength2(
+    pairs: Linear<UTF8.ValidUTF8Bytes, UTF8.ValidUTF8Bytes>
+  ):
+    (ret: nat)
+    ensures |pairs| == 0 ==> ret == 0
+  {
+    if |pairs| == 0 then 0
+    else
+      LinearLength2(Seq.DropLast(pairs)) + PairLength(Seq.Last(pairs))
+  }
+
+  function method PairLength(
+    pair: Pair<UTF8.ValidUTF8Bytes, UTF8.ValidUTF8Bytes>
+  ):
+    (ret: nat)
+  {
+    2 + |pair.key| + 2 + |pair.value|
+  }
+
+}
