src/Util/Sets.dfy
@@ -2,11 +2,19 @@
 // SPDX-License-Identifier: Apache-2.0
 
 include "../StandardLibrary/StandardLibrary.dfy"
+include "../../libraries/src/Collections/Sequences/Seq.dfy"
 
 module {:extern "Sets"} Sets {
   import opened StandardLibrary
+  import Seq
 
-  method {:extern "SetToOrderedSequence"} ComputeSetToOrderedSequence<T(==)>(s: set<seq<T>>, less: (T, T) -> bool) returns (res: seq<seq<T>>)
+  function method {:extern "SetToOrderedSequence"} ComputeSetToOrderedSequence<T(==)>(
+    s: set<seq<T>>,
+    less: (T, T) -> bool
+  )
+    :(res: seq<seq<T>>)
     requires Trichotomous(less) && Transitive(less)
     ensures res == SetToOrderedSequence(s, less)
+    // The seq came from the set
+    ensures Seq.HasNoDuplicates(res)
 }
